Ideal : Step 1 : todo, step 2 : 70%, step 3 : todo

sha3/proof/smart_counter/Gconcl_list.ec
@@ -1,18 +1,15 @@
 pragma -oldip.
 require import Core Int Real RealExtra StdOrder Ring StdBigop IntExtra.
 require import List FSet NewFMap Utils Common SLCommon RndO FelTactic Mu_mem.
-require import DProd Dexcepted BlockSponge.
+require import DProd Dexcepted BlockSponge Gconcl.
 (*...*) import Capacity IntOrder Bigreal RealOrder BRA.
 
 require (*--*) Handle.
-
-
 
 (*** THEORY PARAMETERS ***)
 (** Validity of Functionality Queries **)
 op valid: block list -> bool = valid_block.
 axiom valid_spec p: valid p => p <> [].
-
 
 clone export Handle as Handle0.
 
@@ -72,7 +69,6 @@ module NIndif (F : FUNCTIONALITY, P : PRIMITIVE, D : DISTINGUISHER) = {
 
 
 module P = Perm.
-
 
 
 section Real_Ideal.
@@ -210,24 +206,38 @@ section Real_Ideal.
   local lemma equiv_sponge (D <: DISTINGUISHER {P, Redo, C, SLCommon.C}) :
     equiv [ GReal(A(D)).main
       ~ NIndif(Squeeze(SqueezelessSponge(P)),P,DRestr(D)).main
-      : ={glob D} ==> ={res, glob D, glob P, C.c} /\ SLCommon.C.c{1} <= C.c{2}].
+      : ={glob D} ==> ={res, glob D, glob P, C.c} /\ SLCommon.C.c{1} <= C.c{2} <= max_size].
   proof.
   proc;inline*;sp;wp.
-  call(: ={Redo.prefixes, glob P, C.c} /\
+  call(: ={Redo.prefixes, glob P, C.c} /\ C.c{1} <= max_size /\
     INV_Real SLCommon.C.c{1} C.c{2} Perm.m{1} Perm.mi{1} Redo.prefixes{1});auto;last first.
-  + by progress;1:(split=>//=;1:split;smt(dom0 in_fset0 dom_set in_fsetU1 getP map0P));case:H0=>//=. 
+  + progress. 
+    + exact max_ge0.
+    + by split=>//=;1:split;smt(dom0 in_fset0 dom_set in_fsetU1 getP map0P).
+    by case:H2=>//=. 
   + by proc;inline*;auto;sp;if;auto;sp;if;auto;
       smt(INV_Real_addm_mi INV_Real_incr supp_dexcepted).
   + proc;inline*;auto;sp;if;auto;sp;if;auto;progress.
     + apply INV_Real_incr=>//=.
       apply INV_Real_addm_mi=>//=.
-      + case:H=>H_c H_m_p H_invm;rewrite (invm_dom_rng _ _ H_invm)//=. 
-        by move:H2;rewrite supp_dexcepted.
-      case:H=>H_c H_m_p H_invm;cut<-//:=(invm_dom_rng Perm.mi{2} Perm.m{2}). 
+      + case:H0=>H_c H_m_p H_invm;rewrite (invm_dom_rng _ _ H_invm)//=. 
+        by move:H3;rewrite supp_dexcepted.
+      case:H0=>H_c H_m_p H_invm;cut<-//:=(invm_dom_rng Perm.mi{2} Perm.m{2}). 
       by rewrite invmC.
     + exact INV_Real_incr.
   + proc;inline*;sp;if;auto.
-    swap 6;wp;sp=>/=;if;auto;last by progress;split;case:H=>//=;smt(size_ge0).
+    swap 6;wp;sp=>/=;if;auto;last by progress;split;case:H0=>//=;smt(size_ge0).
+    conseq(: p{2} = bl{2} /\ n{2} = nb{2} /\ lres{2} = [] /\ b{2} = b0 /\
+    i{2} = 0 /\ p{1} = bl{1} /\ n{1} = nb{1} /\ lres{1} = [] /\ b{1} = b0 /\
+    i{1} = 0 /\ z{2} = [] /\ z{1} = [] /\ ={bl, nb} /\ ={Redo.prefixes} /\
+    ={Perm.mi, Perm.m} /\ ={C.c} /\
+    INV_Real SLCommon.C.c{1} C.c{2} Perm.m{1} Perm.mi{1} Redo.prefixes{1} /\
+    C.c{1} + size bl{1} + max (nb{1} - 1) 0 <= max_size /\ valid p{1}
+  ==> ={lres} /\ ={Redo.prefixes} /\ ={Perm.mi, Perm.m} /\
+    C.c{1} + size bl{1} + max (nb{1} - 1) 0 =
+    C.c{2} + size bl{2} + max (nb{2} - 1) 0 /\
+    INV_Real SLCommon.C.c{1} (C.c{2} + size bl{2} + max (nb{2} - 1) 0)
+    Perm.m{1} Perm.mi{1} Redo.prefixes{1});progress.
     sp.
     seq 2 2:(={i,n,p,lres,nb,bl,b,glob P,glob C,glob Redo}
            /\  INV_Real SLCommon.C.c{1} (C.c{2} + size bl{2})
@@ -565,23 +575,34 @@ section Real_Ideal.
   local lemma squeeze_squeezeless (D <: DISTINGUISHER {P, Redo, C, SLCommon.C}) :
     equiv [ NIndif(Squeeze(SqueezelessSponge(P)),P,DRestr(D)).main
         ~ RealIndif(Sponge,P,DRestr(D)).main
-        : ={glob D} ==> ={res, glob P, glob D, C.c}].
+        : ={glob D} ==> ={res, glob P, glob D, C.c} /\ C.c{1} <= max_size].
   proof.
   proc;inline*;sp;wp. 
-  call(: ={glob Perm,C.c}
+  call(: ={glob Perm,C.c} /\ C.c{1} <= max_size
       /\ INV_Real 0 C.c{1} Perm.m{1} Perm.mi{1} Redo.prefixes{1});auto;last first.
-  + progress. 
+  + progress.
+    + exact max_ge0.
     split=>//=;1:split=>//=;smt(getP dom0 map0P in_fset0 dom_set in_fsetU1). 
   + proc;inline*;auto;sp;if;auto;sp;if;auto;progress.
-    - by rewrite INV_Real_addm_mi;2..:smt(supp_dexcepted);split;case:H=>//=;smt().
-    - by split;case:H=>//=;smt().
+    - by rewrite INV_Real_addm_mi;2..:smt(supp_dexcepted);split;case:H0=>//=;smt().
+    - by split;case:H0=>//=;smt().
   + proc;inline*;auto;sp;if;auto;sp;if;auto;progress.
-    - rewrite INV_Real_addm_mi;1: by split;case:H=>//=;smt().
-      * case:H;smt(invm_dom_rng invmC supp_dexcepted).
-      case:H;smt(invm_dom_rng invmC supp_dexcepted).
-    - by split;case:H=>//=;smt(). 
+    - rewrite INV_Real_addm_mi;1: by split;case:H0=>//=;smt().
+      * case:H0;smt(invm_dom_rng invmC supp_dexcepted).
+      case:H0;smt(invm_dom_rng invmC supp_dexcepted).
+    - by split;case:H0=>//=;smt(). 
   proc;inline*;sp;auto;if;auto;sp;if;auto;
-    last by progress;split;case:H=>//=;smt(size_ge0).
+    last by progress;split;case:H0=>//=;smt(size_ge0).
+  conseq(: (exists (c_R : int),
+      C.c{2} = c_R + size bl{2} + max (nb{2} - 1) 0 /\ xs{2} = bl{2} /\
+      n{2} = nb{2} /\ z0{2} = [] /\ sc{2} = c0 /\ sa{2} = b0 /\ i{2} = 0 /\
+      exists (c_L : int), C.c{1} = c_L + size bl{1} + max (nb{1} - 1) 0 /\
+      p{1} = bl{1} /\ n{1} = nb{1} /\ lres{1} = [] /\ b{1} = b0 /\
+      i{1} = 0 /\ z{2} = [] /\ z{1} = [] /\ ={bl, nb} /\
+      ={Perm.mi, Perm.m} /\ c_L = c_R /\
+      INV_Real 0 c_L Perm.m{1} Perm.mi{1} Redo.prefixes{1} /\ valid p{1})
+    ==> lres{1} = z0{2} /\ ={Perm.mi, Perm.m} /\ ={C.c} /\
+      INV_Real 0 C.c{1} Perm.m{1} Perm.mi{1} Redo.prefixes{1});1,2:smt().
   sp.
   seq 2 1 : (={glob P, i, n, C.c,sa,sc}
     /\ b{1} = sa{2} /\ Redo.prefixes.[p]{1} = Some (sa,sc){2}
@@ -805,14 +826,305 @@ section Real_Ideal.
   qed. 
 
 
+
   local lemma pr_real (D <: DISTINGUISHER{SLCommon.C, C, Perm, Redo}) &m :
-      Pr [ GReal(A(D)).main() @ &m : res ] =
-      Pr [ RealIndif(Sponge,P,DRestr(D)).main() @ &m : res ].
+      Pr [ GReal(A(D)).main() @ &m : res /\ SLCommon.C.c <= max_size] <=
+      Pr [ RealIndif(Sponge,P,DRestr(D)).main() @ &m : res].
   proof.
   cut->:Pr [ RealIndif(Sponge, P, DRestr(D)).main() @ &m : res ] =
-        Pr [ NIndif(Squeeze(SqueezelessSponge(P)),P,DRestr(D)).main() @ &m : res ].
+        Pr [ NIndif(Squeeze(SqueezelessSponge(P)),P,DRestr(D)).main() @ &m : res /\ C.c <= max_size ].
   + by rewrite eq_sym;byequiv (squeeze_squeezeless D)=>//=.
-  by byequiv (equiv_sponge D)=>//=.
+  byequiv (equiv_sponge D)=>//=;progress.
+  qed.
+
+
+  print Real_Ideal.
+
+  print SLCommon.SIMULATOR.
+
+  print Last.
+
+  module SimLast (S : SLCommon.SIMULATOR) (F : DFUNCTIONALITY) = S(Last(F)).
+
+  op (<=) (m1 m2 : (block list, 'b) fmap) = 
+    forall x, x <> [] => x \in dom m1 => m1.[x] = m2.[x].
+
+  local lemma leq_add_nin (m1 m2 : (block list, 'b) fmap) (x : block list) (y : 'b):
+      m1 <= m2 => 
+      ! x \in dom m2 =>
+      m1 <= m2.[x <- y].
+  proof.
+  move=>h_leq H_n_dom a H_a_dom;rewrite getP/=;smt(in_dom).
+  qed.
+
+
+  local lemma leq_add_in (m1 m2 : (block list, 'b) fmap) (x : block list) :
+      m1 <= m2 => 
+      x \in dom m2 =>
+      m1.[x <- oget m2.[x]] <= m2.
+  proof.
+  move=>h_leq H_n_dom a H_a_dom;rewrite getP/=;smt(in_dom getP).
+  qed.
+
+  local lemma leq_nin_dom (m1 m2 : (block list, 'b) fmap) (x : block list) :
+      m1 <= m2 =>
+      x <> [] =>
+      ! x \in dom m2 => ! x \in dom m1 by smt(in_dom).
+
+  local lemma prefixe_leq1 (l : block list) (m : (block list,block) fmap) i :
+      0 <= i =>
+      format l (i+1) \in dom m =>
+      size (format l (i+1)) <= prefixe (format l (i+1+1)) 
+        (get_max_prefixe (format l (i+1+1)) (elems (dom m))) <= size (format l (i+1+1)).
+  proof. 
+  rewrite memE;move=>hi0 H_dom. 
+  cut->:(format l (i + 1 + 1)) = format l (i + 1) ++ [b0].
+  + by rewrite/format/=-2!(addzA _ 1 (-1))//=nseqSr//-cats1 catA. 
+  cut:=prefixe_leq_prefixe_cat_size (format l (i + 1))[b0](elems (dom m)).
+  rewrite (prefixe_get_max_prefixe_eq_size _ _ H_dom)//=.
+  rewrite (size_cat _ [b0])/=;pose x:= format _ _.
+  cut:=get_max_prefixe_max (x ++ [b0]) _ _ H_dom.
+  cut->:prefixe (x ++ [b0]) (format l (i + 1)) = size x
+    by rewrite prefixeC-{1}(cats0 (format l (i+1)))/x prefixe_cat//=. 
+  smt(prefixe_sizel size_cat prefixe_ge0 ).
+  qed.
+
+  local lemma prefixe_le1 (l : block list) (m : (block list,block) fmap) i :
+      0 <= i =>
+      format l (i+1) \in dom m =>
+      size (format l (i+1+1)) - prefixe (format l (i+1+1)) 
+        (get_max_prefixe (format l (i+1+1)) (elems (dom m))) <= 1.
+  proof. 
+  smt(prefixe_leq1 size_ge0 size_cat size_nseq).
+  qed.
+
+  local lemma leq_add2  (m1 m2 : (block list, 'b) fmap) (x : block list) (y : 'b) :
+      m1 <= m2 => 
+      ! x \in dom m2 =>
+      m1.[x <- y] <= m2.[x <- y] by smt(in_dom getP dom_set in_fsetU1).
+
+
+  local equiv ideal_equiv (D <: DISTINGUISHER{SLCommon.C, C, IF, BIRO.IRO, S}) :
+      SLCommon.IdealIndif(IF, S, SLCommon.DRestr(A(D))).main
+      ~
+      SLCommon.IdealIndif(IF, S, A(D)).main
+      :
+      ={glob D} ==> ={glob D, res}.
+  proof.
+  proc;inline*;auto;sp.
+  call(: ={glob IF, glob S, glob A} /\ SLCommon.C.c{1} <= C.c{1}
+      /\ SLCommon.C.queries{1} <= F.RO.m{2});auto;last first.
+  + progress.
+    by move=>x;rewrite getP/=dom_set in_fsetU1 dom0 in_fset0//==>->.
+  + proc;inline*;sp;if;auto;sp;rcondt{1}1;1:auto=>/#;sp;if=>//=;2:auto=>/#.
+    wp 7 6;conseq(:_==> ={y} /\ ={F.RO.m} /\ ={S.paths, S.mi, S.m}
+        /\ SLCommon.C.queries{1} <= F.RO.m{2});1:smt().
+    if;auto;smt(leq_add_nin).
+  + by proc;inline*;sp;if;auto;sp;rcondt{1}1;1:auto=>/#;sp;if;auto;smt().
+  proc;inline*;sp;if;auto;swap 6;auto;sp;if;auto;2:smt(size_ge0).
+  case(0 < n{1});last first.
+  + sp;rcondf{1}3;2:rcondf{2}4;1,2:auto.
+     - by if;auto;if;auto.
+    by if{1};2:auto;1:if{1};auto;
+     smt(prefixe_ge0 leq_add_in DBlock.dunifin_ll in_dom size_ge0 getP leq_add2).
+  splitwhile{1}5: i + 1 < n;splitwhile{2}5: i + 1 < n.
+  rcondt{1}6;2:rcondt{2}6;auto.
+  * by while(i < n);auto;sp;if;auto;sp;if;auto;if;auto.
+  * by while(i < n);auto;sp;if;auto;sp;if;auto;if;auto.
+  rcondf{1}8;2:rcondf{2}8;auto.
+  * while(i < n);auto.
+      by sp;if;auto;sp;if;auto;if;auto.
+    sp;if;auto;2:smt();if;auto;smt().
+  * while(i < n);auto;2:smt();sp;if;auto;sp;if;auto;if;auto.
+  rcondf{1}8;2:rcondf{2}8;auto.
+  * while(i < n);auto.
+      by sp;if;auto;sp;if;auto;if;auto.
+    sp;if;auto;2:smt();if;auto;smt().
+  * by while(i < n);auto;2:smt();sp;if;auto;sp;if;auto;if;auto.
+  conseq(:_==> ={b,lres,F.RO.m,S.paths,S.mi,S.m}
+        /\ i{1} = n{1} - 1
+        /\ SLCommon.C.c{1} <= C.c{1} + size bl{1} + i{1}
+        /\ SLCommon.C.queries{1} <= F.RO.m{2});1:smt().
+  while(={lres,F.RO.m,S.paths,S.mi,S.m,i,n,p,nb,b,bl}
+        /\ 0 <= i{1} <= n{1} - 1
+        /\ SLCommon.C.queries.[format p (i+1)]{1} = Some b{1}
+        /\ p{1} = bs{1} /\ valid p{1} /\ p{1} = bl{1}
+        /\ C.c{1} + size p{1} + n{1} - 1 <= max_size
+        /\ SLCommon.C.c{1} <= C.c{1} + size bl{1} + i{1}
+        /\ SLCommon.C.queries{1} <= F.RO.m{2});progress.
+  sp;rcondt{1}1;2:rcondt{2}1;1,2:auto;sp.
+  case((x0 \in dom F.RO.m){2});last first.
+  * rcondt{2}2;1:auto;rcondt{1}1;1:(auto;smt(leq_nin_dom size_cat size_eq0 size_nseq valid_spec)).
+    rcondt{1}1;1:auto;1:smt(prefixe_le1 in_dom size_cat size_nseq). 
+    sp;rcondt{1}2;auto;progress.
+    - smt().
+    - smt().
+    - by rewrite!getP/=.
+    - smt(prefixe_le1 in_dom).
+    - by rewrite!getP/=oget_some leq_add2//=.
+  if{1}.
+  * rcondt{1}1;1:auto;1:smt(prefixe_le1 in_dom size_cat size_nseq). 
+    sp;rcondf{1}2;2:rcondf{2}2;auto;progress.
+    - smt().
+    - smt().
+    - by rewrite!getP/=.
+    - smt(prefixe_ge0 prefixe_le1 in_dom).
+    - smt(leq_add_in in_dom).
+  rcondf{2}2;auto;progress.
+  - smt(DBlock.dunifin_ll).
+  - smt().
+  - smt().
+  - smt().
+  - smt(set_eq in_dom).
+  - smt().
+  sp;conseq(:_==> ={F.RO.m,b}
+        /\ SLCommon.C.queries.[p]{1} = Some b{1}
+        /\ SLCommon.C.c{1} <= C.c{1} + size bl{1}
+        /\ SLCommon.C.queries{1} <= F.RO.m{2});progress.
+  - smt().
+  - smt(nseq0 cats0).
+  - smt(size_ge0).
+  - smt().
+  case(p{2} \in dom F.RO.m{2}).
+  + rcondf{2}2;1:auto.
+    sp;if{1}.
+    - rcondt{1}1;1:auto;1:smt(prefixe_ge0).
+      sp;rcondf{1}2;auto;progress.
+      * by rewrite!getP/=. 
+      * smt(prefixe_ge0).
+      * smt(leq_add_in in_dom).
+    auto;progress.
+    - exact DBlock.dunifin_ll.
+    - smt(in_dom).
+    - smt(in_dom get_oget).
+    - smt(size_ge0).
+  rcondt{1}1;1:auto;1:smt(leq_nin_dom in_dom).
+  rcondt{1}1;1:auto;1:smt(prefixe_ge0).
+  sp;auto;progress.
+  + by rewrite!getP/=.
+  + smt(prefixe_ge0).
+  + rewrite getP/=oget_some leq_add2//=.
+  + by rewrite!getP/=.
+  + smt(prefixe_ge0).
+  + exact leq_add_in.
+  qed.
+
+
+  local module IF'(F : F.RO) = {
+    proc init = F.init
+    proc f (x : block list) : block = {
+      var b : block <- b0;
+      var i : int <- 0;
+      var p,n;
+      (p,n) <- parse x;
+      if (valid p) {
+        while (i < n) {
+          i <- i + 1;
+          F.sample(format p i);
+        }
+        b <@ F.get(x);
+      }
+      return b;
+    }
+  }.
+
+
+  local module SampleFirst (I : BIRO.IRO) = {
+    proc init = I.init
+    proc f (m : block list, k : int) = {
+      var r : block list <- [];
+      if (k <= 0) {
+        I.f(m,1);
+      } else {
+        r <- I.f(m,k);
+      }
+      return r;
+    }
+  }.
+
+
+  axiom valid_gt0 x : valid (parse x).`1 => 0 < (parse x).`2.
+  axiom valid_uniq p1 p2 n1 n2 :
+      valid p1 => valid p2 => format p1 n1 = format p2 n2 => p1 = p2 /\ n1 = n2.
+
+  op inv_map (m1 : (block list, block) fmap) (m2 : (block list * int, block) fmap) =
+      (forall p n, valid p => (p,n) \in dom m2 <=> format p (n+1) \in dom m1)
+      /\ (forall x, x \in dom m1 <=> ((parse x).`1,(parse x).`2-1) \in dom m2)
+      /\ (forall p n, valid p => m2.[(p,n-1)] = m1.[format p n])
+      /\ (forall x, m1.[x] = m2.[((parse x).`1,(parse x).`2-1)]).
+
+print BIRO.
+
+  local equiv Ideal_equiv (D <: DISTINGUISHER{SLCommon.C, C, IF, BIRO.IRO, S}) :
+      SLCommon.IdealIndif(IF'(F.RO), S, A(D)).main
+      ~
+      IdealIndif(SampleFirst(BIRO.IRO), SimLast(S), DRestr(D)).main
+      :
+      ={glob D} ==> ={glob D, res}.
+  proof.
+  proc;inline*;auto;sp.
+  call(: ={glob S, glob C} /\ inv_map F.RO.m{1} BIRO.IRO.mp{2});auto;last first.
+  + smt(dom0 in_fset0 map0P).
+  + proc;inline*;auto;sp;if;1,3:auto;sp;if;1,3:auto;if;1,3:auto;sp.
+    if{1};last by auto;if{2};auto;sp;rcondf{2}1;auto;smt().
+    rcondf{2}1;1:auto;1:smt(parse_valid valid_gt0).
+    sp;rcondt{2}1;1:auto=>/#.
+    seq 8 6 : (={x,y,glob S,C.c} /\ inv_map F.RO.m{1} BIRO.IRO.mp{2});
+      last by conseq(:_==> ={z,glob S,C.c});progress;sim;progress.
+    wp;rnd;auto=>//=;rcondt{1}1;2:rcondt{2}1;1,2:by auto;smt(valid_gt0).
+    sp;conseq(:_==> (x0{1} \in dom F.RO.m{1})
+          /\ inv_map F.RO.m{1} BIRO.IRO.mp{2}
+          /\ oget F.RO.m.[x0]{1} = last b0 bs0{2});
+      1:smt(DBlock.dunifin_ll getP dom_set in_fsetU1). 
+    conseq(:_==> format p0{1} i{1} \in dom F.RO.m{1}
+          /\ inv_map F.RO.m{1} BIRO.IRO.mp{2}
+          /\ i{1} = n{1}
+          /\ oget F.RO.m.[format p0{1} i{1}]{1} = last b0 bs0{2});1:smt().
+    while((i,n){1} = (i0,n0){2} /\ x1{2} = p0{1} /\ valid p0{1}
+          /\ format p0{1} i{1} \in dom F.RO.m{1}
+          /\ inv_map F.RO.m{1} BIRO.IRO.mp{2} /\ 0 < i{1} <= n{1}
+          /\ oget F.RO.m.[format p0{1} i{1}]{1} = last b0 bs0{2});progress.
+    - sp;if{2}.
+      * rcondt{1}2;1:auto=>/#;wp;rnd;skip;smt(dom_set in_fsetU1 valid_uniq
+            formatK parseK getP in_dom last_rcons).
+      by rcondf{1}2;auto;smt(dom_set in_fsetU1 valid_uniq formatK parseK getP 
+            in_dom DBlock.dunifin_ll last_rcons).
+    sp;if{2}.
+    - rcondt{1}2;1:auto=>/#;wp;rnd;skip;smt(dom_set in_fsetU1 valid_uniq 
+            formatK parseK getP in_dom last_rcons valid_gt0).
+    by rcondf{1}2;auto;smt(dom_set in_fsetU1 valid_uniq formatK parseK getP 
+          in_dom DBlock.dunifin_ll last_rcons valid_gt0).
+  + by proc;inline*;auto;sp;if;auto;sp;if;auto.
+  proc;inline*;auto;sp;if;auto;sp.
+  if{2};sp.
+  + if;auto;sp;rcondt{1}1;1:auto;1:smt(parse_valid).
+    rcondt{1}1;auto;1:smt(parse_valid);sp.
+    rcondf{1}3;auto;1:smt(parse_valid);sp.
+    rcondf{1}5;auto;1:smt(dom_set in_fsetU1 nseq0 cats0 parse_valid).
+    rcondt{2}1;auto;rcondf{2}7;1:by auto;sp;if;auto.
+    swap{1}4 3;auto;conseq(:_==> lres{1} = bs{2} /\ ={S.paths, S.mi, S.m}
+        /\ ={C.c} /\ inv_map F.RO.m{1} BIRO.IRO.mp{2});1:smt(DBlock.dunifin_ll).
+    rcondf{1}6;1:auto;1:smt(dom_set in_fsetU1 nseq0 cats0 parse_valid).
+    sp;if{2}.
+    - by rcondt{1}2;auto;smt(parse_valid dom_set in_fsetU1 valid_uniq formatK
+          parseK getP in_dom DBlock.dunifin_ll last_rcons).
+    rcondf{1}2;auto;smt(parse_valid dom_set in_fsetU1 valid_uniq formatK parseK
+        getP in_dom DBlock.dunifin_ll last_rcons).
+  if;auto;sp;rcondt{1}1;auto;1:smt(parse_valid).
+  rcondt{1}1;auto;1:smt(parse_valid);sp.
+  rcondf{1}3;auto;1:smt(parse_valid).
+  rcondf{1}5;auto;1:smt(dom_set in_fsetU1 nseq0 cats0 parse_valid).
+  swap{1}4 3;auto;conseq(:_==> lres{1} = bs0{2} /\ ={S.paths, S.mi, S.m}
+      /\ ={C.c} /\ inv_map F.RO.m{1} BIRO.IRO.mp{2});1:smt(DBlock.dunifin_ll).
+  rcondt{1}6;1:auto=>/#.
+  rcondt{2}1;1:auto=>/#.
+  (* TODO *)
+
+    rcondt{2}1;auto;rcondf{2}7;1:by auto;sp;if;auto.
+  rcondf{1}7;auto.
+  + while
+
+
   qed.
 
   (* TODO : Ideal *)
